# CBMS-2016-07

**题目来源**：[[文字版题库/CBMS/2016#Problem 7|2016#Problem 7]]
**日期**：2024-07-31
**题目主题**：CS-算法-递归时间复杂度

## Solution

Let's analyze the time complexity for each recurrence relation separately.

### 1. $T(n) = T(\lfloor 3n/4 \rfloor) + cn$

For this recurrence, we use the Master Theorem. The recurrence is of the form $T(n) = aT(n/b) + f(n)$.

- Here, $a = 1$, $b = \frac{4}{3}$, and $f(n) = cn$.
- We need to compare $f(n)$ with $n^{\log_b a}$.

First, compute $\log_b a$:

$$

\log_b a = \log_{4/3} 1 = 0

$$

According to the Master Theorem:

- If $f(n) = O(n^c)$ where $c < \log_b a$, then $T(n) = \Theta(n^{\log_b a})$.
- If $f(n) = \Theta(n^{\log_b a})$, then $T(n) = \Theta(n^{\log_b a} \log n)$.
- If $f(n) = \Omega(n^c)$ where $c > \log_b a$ and $af(n/b) \leq kf(n)$ for some $k < 1$ and sufficiently large $n$, then $T(n) = \Theta(f(n))$.

In this case, $f(n) = cn = \Theta(n)$ and $\log_b a = 0$.

Since $c > \log_b a$, we have $T(n) = \Theta(n)$.

Thus, $T(n) \in O(n)$.

### 2. $T(n) = 2T(n - 1) + cn$

To solve this recurrence, we can use the iterative method:

$$

\begin{aligned}

T(n) & = 2T(n - 1) + cn \\

& = 2[2T(n - 2) + c(n - 1)] + cn \\

& = 2^2T(n - 2) + 2c(n - 1) + cn \\

& = 2^2[2T(n - 3) + c(n - 2)] + 2c(n - 1) + cn \\

& = 2^3T(n - 3) + 2^2c(n - 2) + 2c(n - 1) + cn \\

& \vdots \\

& = 2^kT(n - k) + c\sum_{i=0}^{k-1} 2^i(n - i)

\end{aligned}

$$

When $k = n - 1$:

$$

\begin{aligned}

T(n) & = 2^{n-1}T(1) + c\sum_{i=0}^{n-2} 2^i(n - i) \\

& = 2^{n-1}c + c\sum_{i=0}^{n-2} 2^i(n - i) \\

& = 2^{n-1}c + c\left( \sum_{i=1}^{n-1} 2^i (n - i + 1) - \sum_{i=0}^{n-2} 2^i(n - i) \right) \\

& = 2^{n-1}c + c\left( 2^n + \sum_{i=1}^{n-2} 2^i (n - i + 1) - \sum_{i=1}^{n-2} 2^i(n - i)  - n \right) \\

& = 2^{n-1}c + c\left( 2^n - n + \sum_{i=1}^{n-2} 2^i \right) \\

\end{aligned}

$$

The sum $\sum_{i=1}^{n-2} 2^i$ is a geometric series:

$$

\sum_{i=1}^{n-2} 2^i = 2^{n-1} - 2

$$

Thus, $T(n)$ can be approximated by:

$$

T(n) = \Theta(2^n) = O(3^n)

$$

Thus, $T(n) \in O(3^n)$.

### 3. $T(n) = T(n - 1) + c(n^2 + n)$

This is a non-homogeneous linear recurrence relation. We can use the iterative method:

$$

\begin{aligned}

T(n) & = T(n-1) + c(n^2 + n) \\

& = T(n-2) + c((n-1)^2 + (n-1)) + c(n^2 + n) \\

& = T(n-3) + c((n-2)^2 + (n-2)) + c((n-1)^2 + (n-1)) + c(n^2 + n) \\

& \vdots \\

& = T(1) + c \sum_{k=1}^{n-1} (k^2 + k) \\

& = c + c \sum_{k=1}^{n-1} (k^2 + k)

\end{aligned}

$$

The sum $\sum_{k=1}^{n-1} k^2$ is:

$$

\sum_{k=1}^{n-1} k^2 = \frac{(n-1)n(2n-1)}{6}

$$

And the sum $\sum_{k=1}^{n-1} k$ is:

$$

\sum_{k=1}^{n-1} k = \frac{(n-1)n}{2}

$$

Therefore:

$$

\begin{aligned}

T(n) & = c + c \left( \frac{(n-1)n(2n-1)}{6} + \frac{(n-1)n}{2} \right) \\

& = c + c \left( \frac{(n-1)n(2n-1 + 3)}{6} \right) \\

& = c + c \left( \frac{(n-1)n(2n+2)}{6} \right) \\

& = c + \frac{c(n-1)n(n+1)}{3} \\

& = \Theta(n^3)

\end{aligned}

$$

Thus, $T(n) \in O(n^3)$.

### 4. $T(n) = T(\lfloor n/2 \rfloor) + c$

For this recurrence, we again use the Master Theorem. The recurrence is of the form $T(n) = aT(n/b) + f(n)$.

- Here, $a = 1$, $b = 2$, and $f(n) = c$.
- We need to compare $f(n)$ with $n^{\log_b a}$.

First, compute $\log_b a$:

$$

\log_b a = \log_2 1 = 0

$$

According to the Master Theorem:

- If $f(n) = O(n^c)$ where $c < \log_b a$, then $T(n) = \Theta(n^{\log_b a})$.
- If $f(n) = \Theta(n^{\log_b a})$, then $T(n) = \Theta(n^{\log_b a} \log n)$.
- If $f(n) = \Omega(n^c)$ where $c > \log_b a$ and $af(n/b) \leq kf(n)$ for some $k < 1$ and sufficiently large $n$, then $T(n) = \Theta(f(n))$.

In this case, $f(n) = c = \Theta(1)$ and $\log_b a = 0$.

Since $f(n)$ is $\Theta(n^0)$:

$$

T(n) = \Theta(\log n)

$$

Thus, $T(n) \in O(\log n)$.

### 5. $T(n) = 2T(\lfloor n/2 \rfloor) + cn$

For this recurrence, we use the Master Theorem. The recurrence is of the form $T(n) = aT(n/b) + f(n)$.

- Here, $a = 2$, $b = 2$, and $f(n) = cn$.
- We need to compare $f(n)$ with $n^{\log_b a}$.

First, compute $\log_b a$:

$$

\log_b a = \log_2 2 = 1

$$

According to the Master Theorem:

- If $f(n) = O(n^c)$ where $c < \log_b a$, then $T(n) = \Theta(n^{\log_b a})$.
- If $f(n) = \Theta(n^{\log_b a})$, then $T(n) = \Theta(n^{\log_b a} \log n)$.
- If $f(n) = \Omega(n^c)$ where $c > \log_b a$ and $af(n/b) \leq kf(n)$ for some $k < 1$ and sufficiently large $n$, then $T(n) = \Theta(f(n)$.

In this case, $f(n) = cn = \Theta(n)$ and $\log_b a = 1$.

Since $f(n) = \Theta(n^{\log_b a})$, we have:

$$

T(n) = \Theta(n \log n)

$$

Thus, $T(n) \in O(n \log n)$.

## Summary

- **Recurrence 1**: $T(n) = \Theta(n)$, $T(n) \in O(n)$.
- **Recurrence 2**: $T(n) = \Theta(2^n)$, $T(n) \in O(2^n)$.
- **Recurrence 3**: $T(n) = \Theta(n^3)$, $T(n) \in O(n^3)$.
- **Recurrence 4**: $T(n) = \Theta(\log n)$, $T(n) \in O(\log n)$.
- **Recurrence 5**: $T(n) = \Theta(n \log n)$, $T(n) \in O(n \log n)$.

## 知识点

#主定理 #递归 #复杂度分析

## 解题技巧和信息

对于递归方程的时间复杂度分析，使用主定理是一个强大的工具。主定理适用于形如 $T(n) = aT(n/b) + f(n)$ 的递归式。需要注意 $a, b, f(n)$ 的取值以及 $f(n)$ 和 $n^{\log_b a}$ 的比较来判断最终的时间复杂度。对于不能用主定理的递归式，可以使用展开迭代法逐步分析。

## 重点词汇

- **Recurrence Relation** 递归关系
- **Master Theorem** 主定理
- **Time Complexity** 时间复杂度
- **Logarithm** 对数
- **Big O Notation** 大 O 符号

## 参考资料

1. Thomas H. Cormen, Charles E. Leiserson, Ronald L. Rivest, and Clifford Stein. *Introduction to Algorithms*, 3rd Edition. MIT Press, Chapter 4.
